Add multi-cases exception handler

shift-reset/interpreter/interpreter.v
@@ -9,19 +9,19 @@ Local Unset Elimination Schemes.
 
 Inductive iresult : Type :=
 | RReturn : val -> iresult
-| RShift : (val -> imonad iresult) -> kont2S -> iresult
-| RControl : (val -> imonad iresult) -> kont2C -> iresult
+| RShift : (val -> imonad iresult) -> metakont -> iresult
+| RControl : (val -> imonad iresult) -> metakont -> iresult
 | RRaise : exn -> iresult.
 
 Definition handle_RShift (r : iresult) : imonad iresult :=
   match r with
-  | RShift f ks => f (VKontS ks)
+  | RShift f mk => f (VKontReset mk)
   | _ => imonad_pure r
   end.
 
 Definition handle_RControl (r : iresult) : imonad iresult :=
   match r with
-  | RControl f kc => f (VKontC kc)
+  | RControl f mk => f (VKont mk)
   | _ => imonad_pure r
   end.
 
@@ -179,38 +179,38 @@ Definition interpret_case (a : atom) (f1 f2 : val -> imonad iresult) : imonad ir
   | _ => imonad_throw (TypeError "")
   end.
 
-Definition interpret_reset (k : kont1) (m : imonad iresult) (f : val -> imonad iresult) : imonad iresult :=
+Definition interpret_reset (k : kont) (m : imonad iresult) (f : val -> imonad iresult) : imonad iresult :=
   r <- m >>= handle_RShift;
   match r with
   | RReturn v => f v
   | RShift _ _ => imonad_throw (ControlError "unreachable")
-  | RControl f' kc => imonad_pure (RControl f' (K2CReset kc k))
+  | RControl f' mk => imonad_pure (RControl f' (MKReset mk k))
   | RRaise _ => imonad_pure r
   end.
 
-Definition interpret_prompt (k : kont1) (m : imonad iresult) (f : val -> imonad iresult) : imonad iresult :=
+Definition interpret_prompt (k : kont) (m : imonad iresult) (f : val -> imonad iresult) : imonad iresult :=
   r <- m >>= handle_RControl;
   match r with
   | RReturn v => f v
-  | RShift f' ks => imonad_pure (RShift f' (K2SPrompt ks k))
+  | RShift f' mk => imonad_pure (RShift f' (MKPrompt mk k))
   | RControl _ _ => imonad_throw (ControlError "unreachable")
   | RRaise _ => imonad_pure r
   end.
 
-Definition interpret_try (k : kont1) (m : imonad iresult) (f : val -> imonad iresult) (t : exn_term) (h : exn -> imonad iresult) : imonad iresult :=
+Definition interpret_try (k : kont) (t : exn_term) (m : imonad iresult) (f : val -> imonad iresult) (h : exn -> imonad iresult) : imonad iresult :=
   r <- m;
   match r with
   | RReturn v => f v
-  | RShift f' ks => imonad_map (fun env => RShift f' (K2STry ks (ExnC env t) k)) imonad_ask_env
-  | RControl f' kc => imonad_map (fun env => RControl f' (K2CTry kc (ExnC env t) k)) imonad_ask_env
+  | RShift f' mk => imonad_map (fun env => RShift f' (MKTry mk (ExnC env t) k)) imonad_ask_env
+  | RControl f' mk => imonad_map (fun env => RControl f' (MKTry mk (ExnC env t) k)) imonad_ask_env
   | RRaise exn => h exn
   end.
 
-Definition interpret_shift (k : kont1) (f : env -> val -> imonad iresult) : imonad iresult :=
-  imonad_map (fun env => RShift (f env >=> handle_RShift) (K2SPure k)) imonad_ask_env.
+Definition interpret_shift (k : kont) (f : env -> val -> imonad iresult) : imonad iresult :=
+  imonad_map (fun env => RShift (f env >=> handle_RShift) (MKPure k)) imonad_ask_env.
 
-Definition interpret_control (k : kont1) (f : env -> val -> imonad iresult) : imonad iresult :=
-  imonad_map (fun env => RControl (f env >=> handle_RControl) (K2CPure k)) imonad_ask_env.
+Definition interpret_control (k : kont) (f : env -> val -> imonad iresult) : imonad iresult :=
+  imonad_map (fun env => RControl (f env >=> handle_RControl) (MKPure k)) imonad_ask_env.
 
 Definition interpret_raise (a : atom) : imonad iresult :=
   v <- interpret_atom a;
@@ -225,132 +225,128 @@ Definition with_binder (b : binder) (v : val) (m : imonad iresult) : imonad ires
   | BVar x => imonad_local_env (EnvCons x v) m
   end.
 
-Definition with_exn_pattern (p : exn_pattern) (exn : exn) (m : imonad iresult) : imonad iresult :=
+Definition with_exn_pattern (p : pattern) (exn : exn) (m1 m2 : imonad iresult) : imonad iresult :=
   match p with
-  | ExnPAny => m
-  | ExnPVar x => imonad_local_env (EnvCons x (VExn exn)) m
-  | ExnPTag tag x =>
-      let (tag', v) := exn in
-      if tag_eq_dec tag tag' then imonad_local_env (EnvCons x v) m else imonad_pure (RRaise exn)
+  | PAny => m1
+  | PVar x => imonad_local_env (EnvCons x (VExn exn)) m1
+  | PTag tag b => let (tag', v) := exn in if tag_eq_dec tag tag' then with_binder b v m1 else m2
   end.
 
-Definition interpreter : Type := kont1 -> term -> imonad iresult.
+Definition interpreter : Type := kont -> term -> imonad iresult.
 
-Definition interpret_term1_with (rec : interpreter) (k : kont1) (t : term1) (v : val) : imonad iresult :=
+Definition interpret_term1_with (rec : interpreter) (k : kont) (t : term1) (v : val) : imonad iresult :=
   let (b, t') := t in with_binder b v (rec k t').
 
-Definition interpret_term2_with (rec : interpreter) (k : kont1) (t : term2) (v1 v2 : val) : imonad iresult :=
+Definition interpret_term2_with (rec : interpreter) (k : kont) (t : term2) (v1 v2 : val) : imonad iresult :=
   let (b1, b2, t') := t in with_binder b1 v1 (with_binder b2 v2 (rec k t')).
 
-Definition interpret_exn_term_with (rec : interpreter) (k : kont1) (t : exn_term) (exn : exn) : imonad iresult :=
-  let (p, t') := t in with_exn_pattern p exn (rec k t').
-
-Definition interpret_clo1_with (rec : interpreter) (k : kont1) (c : clo1) (v : val) : imonad iresult :=
-  let (env, t) := c in imonad_local_env (fun _ => env) (interpret_term1_with rec k t v).
-
-Definition interpret_clo2_with (rec : interpreter) (k : kont1) (c : clo2) (v1 v2 : val) : imonad iresult :=
-  let (env, t) := c in imonad_local_env (fun _ => env) (interpret_term2_with rec k t v1 v2).
-
-Definition interpret_exn_clo_with (rec : interpreter) (k : kont1) (c : exn_clo) (exn : exn) : imonad iresult :=
-  let (env, t) := c in imonad_local_env (fun _ => env) (interpret_exn_term_with rec k t exn).
-
-Definition interpret_kont1_with (rec : interpreter) (k : kont1) (v : val) : imonad iresult :=
-  match k with
-  | K1Nil => imonad_pure (RReturn v)
-  | K1Cons c k' => interpret_clo1_with rec k' c v
+Fixpoint interpret_exn_term_with (rec : interpreter) (k : kont) (t : exn_term) (exn : exn) : imonad iresult :=
+  match t with
+  | ExnTBase p t' => with_exn_pattern p exn (rec k t') (imonad_pure (RRaise exn))
+  | ExnTCons p t1 t2 => with_exn_pattern p exn (rec k t1) (interpret_exn_term_with rec k t2 exn)
   end.
 
-Definition interpret_K2Reset_with (rec : interpreter) (k : kont1) (m : imonad iresult) : imonad iresult :=
-  interpret_reset k m (interpret_kont1_with rec k).
+Definition interpret_clo1_with (rec : interpreter) (k : kont) (c : clo1) (v : val) : imonad iresult :=
+  let (env, t) := c in imonad_local_env (fun _ => env) (interpret_term1_with rec k t v).
 
-Definition interpret_K2Prompt_with (rec : interpreter) (k : kont1) (m : imonad iresult) : imonad iresult :=
-  interpret_prompt k m (interpret_kont1_with rec k).
+Definition interpret_clo2_with (rec : interpreter) (k : kont) (c : clo2) (v1 v2 : val) : imonad iresult :=
+  let (env, t) := c in imonad_local_env (fun _ => env) (interpret_term2_with rec k t v1 v2).
 
-Definition interpret_K2Try_with (rec : interpreter) (k : kont1) (m : imonad iresult) (c : exn_clo) : imonad iresult :=
+Definition interpret_exn_clo_with (rec : interpreter) (k : kont) (c : exn_clo) (exn : exn) : imonad iresult :=
+  let (env, t) := c in imonad_local_env (fun _ => env) (interpret_exn_term_with rec k t exn).
+
+Definition interpret_kont_with (rec : interpreter) (k : kont) (v : val) : imonad iresult :=
+  match k with
+  | KNil => imonad_pure (RReturn v)
+  | KCons c k' => interpret_clo1_with rec k' c v
+  end.
+
+Definition interpret_K2Reset_with (rec : interpreter) (k : kont) (m : imonad iresult) : imonad iresult :=
+  interpret_reset k m (interpret_kont_with rec k).
+
+Definition interpret_K2Prompt_with (rec : interpreter) (k : kont) (m : imonad iresult) : imonad iresult :=
+  interpret_prompt k m (interpret_kont_with rec k).
+
+Definition interpret_K2Try_with (rec : interpreter) (k : kont) (m : imonad iresult) (c : exn_clo) : imonad iresult :=
   r <- m;
   match r with
-  | RReturn v => interpret_kont1_with rec k v
-  | RShift f ks => imonad_pure (RShift f (K2STry ks c k))
-  | RControl f kc => imonad_pure (RControl f (K2CTry kc c k))
+  | RReturn v => interpret_kont_with rec k v
+  | RShift f mk => imonad_pure (RShift f (MKTry mk c k))
+  | RControl f mk => imonad_pure (RControl f (MKTry mk c k))
   | RRaise exn => interpret_exn_clo_with rec k c exn
   end.
 
-Fixpoint interpret_kont2S_with (rec : interpreter) (ks : kont2S) (v : val) : imonad iresult :=
-  match ks with
-  | K2SPure k => interpret_kont1_with rec k v
-  | K2SPrompt ks' k => interpret_K2Prompt_with rec k (interpret_kont2S_with rec ks' v)
-  | K2STry ks' c k => interpret_K2Try_with rec k (interpret_kont2S_with rec ks' v) c
+Fixpoint interpret_metakont_with (rec : interpreter) (mk : metakont) (v : val) : imonad iresult :=
+  match mk with
+  | MKPure k => interpret_kont_with rec k v
+  | MKReset mk' k => interpret_K2Reset_with rec k (interpret_metakont_with rec mk' v)
+  | MKPrompt mk' k => interpret_K2Prompt_with rec k (interpret_metakont_with rec mk' v)
+  | MKTry mk' c k => interpret_K2Try_with rec k (interpret_metakont_with rec mk' v) c
   end.
 
-Fixpoint interpret_kont2C_with (rec : interpreter) (kc : kont2C) (v : val) : imonad iresult :=
-  match kc with
-  | K2CPure k => interpret_kont1_with rec k v
-  | K2CReset kc' k => interpret_K2Reset_with rec k (interpret_kont2C_with rec kc' v)
-  | K2CTry kc' c k => interpret_K2Try_with rec k (interpret_kont2C_with rec kc' v) c
-  end.
-
-Definition interpret_app (rec : interpreter) (k : kont1) (a1 a2 : atom) (f : val -> imonad iresult) : imonad iresult :=
+Definition interpret_app (rec : interpreter) (k : kont) (a1 a2 : atom) (f : val -> imonad iresult) : imonad iresult :=
   v <- interpret_atom a1;
   match v with
   | VFun c => interpret_atom a2 >>= interpret_clo1_with rec k c
   | VFix c => interpret_atom a2 >>= interpret_clo2_with rec k c v
-  | VKontS ks => interpret_reset k (interpret_atom a2 >>= interpret_kont2S_with rec ks) f
-  | VKontC kc => interpret_atom a2 >>= interpret_kont2C_with rec (kont2C_extend kc k)
+  | VKontReset mk => interpret_reset k (interpret_atom a2 >>= interpret_metakont_with rec mk) f
+  | VKont mk => interpret_atom a2 >>= interpret_metakont_with rec (metakont_extend mk k)
   | _ => imonad_throw (TypeError "")
   end.
 
 Set Implicit Arguments.
 
-Inductive term_graph : kont1 -> term -> Prop :=
-| GTAtom k a : kont1_graph k -> term_graph k (TAtom a)
-| GTFun k t' : kont1_graph k -> term_graph k (TFun t')
-| GTFix k t' : kont1_graph k -> term_graph k (TFix t')
-| GTApp k a1 a2 : kont1_graph k -> term_graph k (TApp a1 a2)
-| GTLet k t1 t2 : (forall env, term_graph (K1Cons (C1 env t2) k) t1) -> term_graph k (TLet t1 t2)
+Inductive term_graph : kont -> term -> Prop :=
+| GTAtom k a : kont_graph k -> term_graph k (TAtom a)
+| GTFun k t' : kont_graph k -> term_graph k (TFun t')
+| GTFix k t' : kont_graph k -> term_graph k (TFix t')
+| GTApp k a1 a2 : kont_graph k -> term_graph k (TApp a1 a2)
+| GTLet k t1 t2 : (forall env, term_graph (KCons (C1 env t2) k) t1) -> term_graph k (TLet t1 t2)
 | GTIf k a t1 t2 : term_graph k t1 -> term_graph k t2 -> term_graph k (TIf a t1 t2)
-| GTPrim1 k p a : kont1_graph k -> term_graph k (TPrim1 p a)
-| GTPrim2 k p a1 a2 : kont1_graph k -> term_graph k (TPrim2 p a1 a2)
-| GTPair k a1 a2 : kont1_graph k -> term_graph k (TPair a1 a2)
+| GTPrim1 k p a : kont_graph k -> term_graph k (TPrim1 p a)
+| GTPrim2 k p a1 a2 : kont_graph k -> term_graph k (TPrim2 p a1 a2)
+| GTPair k a1 a2 : kont_graph k -> term_graph k (TPair a1 a2)
 | GTSplit k a t' : term2_graph k t' -> term_graph k (TSplit a t')
-| GTInl k a : kont1_graph k -> term_graph k (TInl a)
-| GTInr k a : kont1_graph k -> term_graph k (TInr a)
+| GTInl k a : kont_graph k -> term_graph k (TInl a)
+| GTInr k a : kont_graph k -> term_graph k (TInr a)
 | GTCase k a t1 t2 : term1_graph k t1 -> term1_graph k t2 -> term_graph k (TCase a t1 t2)
-| GTRef k a : kont1_graph k -> term_graph k (TRef a)
-| GTGet k a : kont1_graph k -> term_graph k (TGet a)
-| GTSet k a1 a2 : kont1_graph k -> term_graph k (TSet a1 a2)
-| GTFree k a : kont1_graph k -> term_graph k (TFree a)
-| GTShift k t' : (forall env, clo1_graph K1Nil (C1 env t')) -> term_graph k (TShift t')
-| GTReset k t' : term_graph K1Nil t' -> kont1_graph k -> term_graph k (TReset t')
-| GTControl k t' : (forall env, clo1_graph K1Nil (C1 env t')) -> term_graph k (TControl t')
-| GTPrompt k t' : term_graph K1Nil t' -> kont1_graph k -> term_graph k (TPrompt t')
-| GTExn k tag a : kont1_graph k -> term_graph k (TExn tag a)
+| GTRef k a : kont_graph k -> term_graph k (TRef a)
+| GTGet k a : kont_graph k -> term_graph k (TGet a)
+| GTSet k a1 a2 : kont_graph k -> term_graph k (TSet a1 a2)
+| GTFree k a : kont_graph k -> term_graph k (TFree a)
+| GTShift k t' : (forall env, clo1_graph KNil (C1 env t')) -> term_graph k (TShift t')
+| GTReset k t' : term_graph KNil t' -> kont_graph k -> term_graph k (TReset t')
+| GTControl k t' : (forall env, clo1_graph KNil (C1 env t')) -> term_graph k (TControl t')
+| GTPrompt k t' : term_graph KNil t' -> kont_graph k -> term_graph k (TPrompt t')
+| GTExn k tag a : kont_graph k -> term_graph k (TExn tag a)
 | GTRaise k a : term_graph k (TRaise a)
-| GTTry k t1 t2 : term_graph K1Nil t1 -> kont1_graph k -> exn_term_graph k t2 -> term_graph k (TTry t1 t2)
-with term1_graph : kont1 -> term1 -> Prop :=
+| GTTry k t1 t2 : term_graph KNil t1 -> kont_graph k -> exn_term_graph k t2 -> term_graph k (TTry t1 t2)
+with term1_graph : kont -> term1 -> Prop :=
 | GT1 k b t' : term_graph k t' -> term1_graph k (T1 b t')
-with term2_graph : kont1 -> term2 -> Prop :=
+with term2_graph : kont -> term2 -> Prop :=
 | GT2 k b1 b2 t' : term_graph k t' -> term2_graph k (T2 b1 b2 t')
-with exn_term_graph : kont1 -> exn_term -> Prop :=
-| GExnT k p t' : term_graph k t' -> exn_term_graph k (ExnT p t')
-with clo1_graph : kont1 -> clo1 -> Prop :=
+with exn_term_graph : kont -> exn_term -> Prop :=
+| GExnTBase k p t' : term_graph k t' -> exn_term_graph k (ExnTBase p t')
+| GExnTCons k p t1 t2 : term_graph k t1 -> exn_term_graph k t2 -> exn_term_graph k (ExnTCons p t1 t2)
+with clo1_graph : kont -> clo1 -> Prop :=
 | GC1 k env t : term1_graph k t -> clo1_graph k (C1 env t)
-with kont1_graph : kont1 -> Prop :=
-| GK1Nil : kont1_graph K1Nil
-| GK1Cons c k' : clo1_graph k' c -> kont1_graph (K1Cons c k').
+with kont_graph : kont -> Prop :=
+| GKNil : kont_graph KNil
+| GKCons c k' : clo1_graph k' c -> kont_graph (KCons c k').
 
-Lemma GTAtom_inv k a : term_graph k (TAtom a) -> kont1_graph k.
+Lemma GTAtom_inv k a : term_graph k (TAtom a) -> kont_graph k.
 Proof. inversion 1; auto. Defined.
 
-Lemma GTFun_inv k t' : term_graph k (TFun t') -> kont1_graph k.
+Lemma GTFun_inv k t' : term_graph k (TFun t') -> kont_graph k.
 Proof. inversion 1; auto. Defined.
 
-Lemma GTFix_inv k t' : term_graph k (TFix t') -> kont1_graph k.
+Lemma GTFix_inv k t' : term_graph k (TFix t') -> kont_graph k.
 Proof. inversion 1; auto. Defined.
 
-Lemma GTApp_inv k a1 a2 : term_graph k (TApp a1 a2) -> kont1_graph k.
+Lemma GTApp_inv k a1 a2 : term_graph k (TApp a1 a2) -> kont_graph k.
 Proof. inversion 1; auto. Defined.
 
-Lemma GTLet_inv k t1 t2 : term_graph k (TLet t1 t2) -> forall env, term_graph (K1Cons (C1 env t2) k) t1.
+Lemma GTLet_inv k t1 t2 : term_graph k (TLet t1 t2) -> forall env, term_graph (KCons (C1 env t2) k) t1.
 Proof. inversion 1; auto. Defined.
 
 Lemma GTIf_inv1 k a t1 t2 : term_graph k (TIf a t1 t2) -> term_graph k t1.
@@ -359,22 +355,22 @@ Proof. inversion 1; auto. Defined.
 Lemma GTIf_inv2 k a t1 t2 : term_graph k (TIf a t1 t2) -> term_graph k t2.
 Proof. inversion 1; auto. Defined.
 
-Lemma GTPrim1_inv k p a : term_graph k (TPrim1 p a) -> kont1_graph k.
+Lemma GTPrim1_inv k p a : term_graph k (TPrim1 p a) -> kont_graph k.
 Proof. inversion 1; auto. Defined.
 
-Lemma GTPrim2_inv k p a1 a2 : term_graph k (TPrim2 p a1 a2) -> kont1_graph k.
+Lemma GTPrim2_inv k p a1 a2 : term_graph k (TPrim2 p a1 a2) -> kont_graph k.
 Proof. inversion 1; auto. Defined.
 
-Lemma GTPair_inv k a1 a2 : term_graph k (TPair a1 a2) -> kont1_graph k.
+Lemma GTPair_inv k a1 a2 : term_graph k (TPair a1 a2) -> kont_graph k.
 Proof. inversion 1; auto. Defined.
 
 Lemma GTSplit_inv k a t' : term_graph k (TSplit a t') -> term2_graph k t'.
 Proof. inversion 1; auto. Defined.
 
-Lemma GTInl_inv k a : term_graph k (TInl a) -> kont1_graph k.
+Lemma GTInl_inv k a : term_graph k (TInl a) -> kont_graph k.
 Proof. inversion 1; auto. Defined.
 
-Lemma GTInr_inv k a : term_graph k (TInr a) -> kont1_graph k.
+Lemma GTInr_inv k a : term_graph k (TInr a) -> kont_graph k.
 Proof. inversion 1; auto. Defined.
 
 Lemma GTCase_inv1 k a t1 t2 : term_graph k (TCase a t1 t2) -> term1_graph k t1.
@@ -383,43 +379,43 @@ Proof. inversion 1; auto. Defined.
 Lemma GTCase_inv2 k a t1 t2 : term_graph k (TCase a t1 t2) -> term1_graph k t2.
 Proof. inversion 1; auto. Defined.
 
-Lemma GTRef_inv k a : term_graph k (TRef a) -> kont1_graph k.
+Lemma GTRef_inv k a : term_graph k (TRef a) -> kont_graph k.
 Proof. inversion 1; auto. Defined.
 
-Lemma GTGet_inv k a : term_graph k (TGet a) -> kont1_graph k.
+Lemma GTGet_inv k a : term_graph k (TGet a) -> kont_graph k.
 Proof. inversion 1; auto. Defined.
 
-Lemma GTSet_inv k a1 a2 : term_graph k (TSet a1 a2) -> kont1_graph k.
+Lemma GTSet_inv k a1 a2 : term_graph k (TSet a1 a2) -> kont_graph k.
 Proof. inversion 1; auto. Defined.
 
-Lemma GTFree_inv k a : term_graph k (TFree a) -> kont1_graph k.
+Lemma GTFree_inv k a : term_graph k (TFree a) -> kont_graph k.
 Proof. inversion 1; auto. Defined.
 
-Lemma GTShift_inv k t' : term_graph k (TShift t') -> forall env, clo1_graph K1Nil (C1 env t').
+Lemma GTShift_inv k t' : term_graph k (TShift t') -> forall env, clo1_graph KNil (C1 env t').
 Proof. inversion 1; auto. Defined.
 
-Lemma GTReset_inv1 k t' : term_graph k (TReset t') -> term_graph K1Nil t'.
+Lemma GTReset_inv1 k t' : term_graph k (TReset t') -> term_graph KNil t'.
 Proof. inversion 1; auto. Defined.
 
-Lemma GTReset_inv2 k t' : term_graph k (TReset t') -> kont1_graph k.
+Lemma GTReset_inv2 k t' : term_graph k (TReset t') -> kont_graph k.
 Proof. inversion 1; auto. Defined.
 
-Lemma GTControl_inv k t' : term_graph k (TControl t') -> forall env, clo1_graph K1Nil (C1 env t').
+Lemma GTControl_inv k t' : term_graph k (TControl t') -> forall env, clo1_graph KNil (C1 env t').
 Proof. inversion 1; auto. Defined.
 
-Lemma GTPrompt_inv1 k t' : term_graph k (TPrompt t') -> term_graph K1Nil t'.
+Lemma GTPrompt_inv1 k t' : term_graph k (TPrompt t') -> term_graph KNil t'.
 Proof. inversion 1; auto. Defined.
 
-Lemma GTPrompt_inv2 k t' : term_graph k (TPrompt t') -> kont1_graph k.
+Lemma GTPrompt_inv2 k t' : term_graph k (TPrompt t') -> kont_graph k.
 Proof. inversion 1; auto. Defined.
 
-Lemma GTExn_inv k tag a : term_graph k (TExn tag a) -> kont1_graph k.
+Lemma GTExn_inv k tag a : term_graph k (TExn tag a) -> kont_graph k.
 Proof. inversion 1; auto. Defined.
 
-Lemma GTTry_inv1 k t1 t2 : term_graph k (TTry t1 t2) -> term_graph K1Nil t1.
+Lemma GTTry_inv1 k t1 t2 : term_graph k (TTry t1 t2) -> term_graph KNil t1.
 Proof. inversion 1; auto. Defined.
 
-Lemma GTTry_inv2 k t1 t2 : term_graph k (TTry t1 t2) -> kont1_graph k.
+Lemma GTTry_inv2 k t1 t2 : term_graph k (TTry t1 t2) -> kont_graph k.
 Proof. inversion 1; auto. Defined.
 
 Lemma GTTry_inv3 k t1 t2 : term_graph k (TTry t1 t2) -> exn_term_graph k t2.
@@ -431,22 +427,28 @@ Proof. inversion 1; auto. Defined.
 Lemma GT2_inv k b1 b2 t' : term2_graph k (T2 b1 b2 t') -> term_graph k t'.
 Proof. inversion 1; auto. Defined.
 
-Lemma GExnT_inv k p t' : exn_term_graph k (ExnT p t') -> term_graph k t'.
+Lemma GExnTBase_inv k p t' : exn_term_graph k (ExnTBase p t') -> term_graph k t'.
+Proof. inversion 1; auto. Defined.
+
+Lemma GExnTCons_inv1 k p t1 t2 : exn_term_graph k (ExnTCons p t1 t2) -> term_graph k t1.
+Proof. inversion 1; auto. Defined.
+
+Lemma GExnTCons_inv2 k p t1 t2 : exn_term_graph k (ExnTCons p t1 t2) -> exn_term_graph k t2.
 Proof. inversion 1; auto. Defined.
 
 Lemma GC1_inv k env t : clo1_graph k (C1 env t) -> term1_graph k t.
 Proof. inversion 1; auto. Defined.
 
-Lemma GK1Cons_inv c k' : kont1_graph (K1Cons c k') -> clo1_graph k' c.
+Lemma GKCons_inv c k' : kont_graph (KCons c k') -> clo1_graph k' c.
 Proof. inversion 1; auto. Defined.
 
-Fixpoint build_term_graph_dep (k : kont1) (G : kont1_graph k) (t : term) : term_graph k t :=
+Fixpoint build_term_graph_dep (k : kont) (G : kont_graph k) (t : term) : term_graph k t :=
   match t with
   | TAtom a => GTAtom a G
   | TFun t' => GTFun t' G
   | TFix t' => GTFix t' G
   | TApp a1 a2 => GTApp a1 a2 G
-  | TLet t1 t2 => GTLet (fun env => build_term_graph_dep (GK1Cons (GC1 env (build_term1_graph_dep G t2))) t1)
+  | TLet t1 t2 => GTLet (fun env => build_term_graph_dep (GKCons (GC1 env (build_term1_graph_dep G t2))) t1)
   | TIf a t1 t2 => GTIf a (build_term_graph_dep G t1) (build_term_graph_dep G t2)
   | TPrim1 p a => GTPrim1 p a G
   | TPrim2 p a1 a2 => GTPrim2 p a1 a2 G
@@ -459,103 +461,108 @@ Fixpoint build_term_graph_dep (k : kont1) (G : kont1_graph k) (t : term) : term_
   | TGet a => GTGet a G
   | TSet a1 a2 => GTSet a1 a2 G
   | TFree a => GTFree a G
-  | TShift t' => GTShift k (fun env => GC1 env (build_term1_graph_dep GK1Nil t'))
-  | TReset t' => GTReset (build_term_graph_dep GK1Nil t') G
-  | TControl t' => GTControl k (fun env => GC1 env (build_term1_graph_dep GK1Nil t'))
-  | TPrompt t' => GTPrompt (build_term_graph_dep GK1Nil t') G
+  | TShift t' => GTShift k (fun env => GC1 env (build_term1_graph_dep GKNil t'))
+  | TReset t' => GTReset (build_term_graph_dep GKNil t') G
+  | TControl t' => GTControl k (fun env => GC1 env (build_term1_graph_dep GKNil t'))
+  | TPrompt t' => GTPrompt (build_term_graph_dep GKNil t') G
   | TExn tag a => GTExn tag a G
   | TRaise a => GTRaise k a
-  | TTry t1 t2 => GTTry (build_term_graph_dep GK1Nil t1) G (build_exn_term_graph_dep G t2)
+  | TTry t1 t2 => GTTry (build_term_graph_dep GKNil t1) G (build_exn_term_graph_dep G t2)
   end
-with build_term1_graph_dep (k : kont1) (G : kont1_graph k) (t : term1) : term1_graph k t :=
+with build_term1_graph_dep (k : kont) (G : kont_graph k) (t : term1) : term1_graph k t :=
   match t with
   | T1 b t' => GT1 b (build_term_graph_dep G t')
   end
-with build_term2_graph_dep (k : kont1) (G : kont1_graph k) (t : term2) : term2_graph k t :=
+with build_term2_graph_dep (k : kont) (G : kont_graph k) (t : term2) : term2_graph k t :=
   match t with
   | T2 b1 b2 t' => GT2 b1 b2 (build_term_graph_dep G t')
   end
-with build_exn_term_graph_dep (k : kont1) (G : kont1_graph k) (t : exn_term) : exn_term_graph k t :=
+with build_exn_term_graph_dep (k : kont) (G : kont_graph k) (t : exn_term) : exn_term_graph k t :=
   match t with
-  | ExnT p t' => GExnT p (build_term_graph_dep G t')
+  | ExnTBase p t' => GExnTBase p (build_term_graph_dep G t')
+  | ExnTCons p t1 t2 => GExnTCons p (build_term_graph_dep G t1) (build_exn_term_graph_dep G t2)
   end.
 
-Definition build_clo1_graph_dep (k : kont1) (G : kont1_graph k) (c : clo1) : clo1_graph k c :=
+Definition build_clo1_graph_dep (k : kont) (G : kont_graph k) (c : clo1) : clo1_graph k c :=
   match c with
   | C1 env t => GC1 env (build_term1_graph_dep G t)
   end.
 
-Fixpoint interpret_term_dep (rec : interpreter) (k : kont1) (t : term) (G : term_graph k t) : imonad iresult :=
+Fixpoint interpret_term_dep (rec : interpreter) (k : kont) (t : term) (G : term_graph k t) : imonad iresult :=
   match t return term_graph k t -> imonad iresult with
-  | TAtom a => fun G => interpret_atom a >>= interpret_kont1_dep rec (GTAtom_inv G)
-  | TFun t' => fun G => interpret_fun t' >>= interpret_kont1_dep rec (GTFun_inv G)
-  | TFix t' => fun G => interpret_fix t' >>= interpret_kont1_dep rec (GTFix_inv G)
-  | TApp a1 a2 => fun G => interpret_app rec k a1 a2 (interpret_kont1_dep rec (GTApp_inv G))
+  | TAtom a => fun G => interpret_atom a >>= interpret_kont_dep rec (GTAtom_inv G)
+  | TFun t' => fun G => interpret_fun t' >>= interpret_kont_dep rec (GTFun_inv G)
+  | TFix t' => fun G => interpret_fix t' >>= interpret_kont_dep rec (GTFix_inv G)
+  | TApp a1 a2 => fun G => interpret_app rec k a1 a2 (interpret_kont_dep rec (GTApp_inv G))
   | TLet t1 t2 => fun G => interpret_let (fun env => interpret_term_dep rec (GTLet_inv G env))
   | TIf a t1 t2 => fun G => interpret_if a (interpret_term_dep rec (GTIf_inv1 G)) (interpret_term_dep rec (GTIf_inv2 G))
-  | TPrim1 p a => fun G => interpret_prim1 p a >>= interpret_kont1_dep rec (GTPrim1_inv G)
-  | TPrim2 p a1 a2 => fun G => interpret_prim2 p a1 a2 >>= interpret_kont1_dep rec (GTPrim2_inv G)
-  | TPair a1 a2 => fun G => interpret_pair a1 a2 >>= interpret_kont1_dep rec (GTPair_inv G)
+  | TPrim1 p a => fun G => interpret_prim1 p a >>= interpret_kont_dep rec (GTPrim1_inv G)
+  | TPrim2 p a1 a2 => fun G => interpret_prim2 p a1 a2 >>= interpret_kont_dep rec (GTPrim2_inv G)
+  | TPair a1 a2 => fun G => interpret_pair a1 a2 >>= interpret_kont_dep rec (GTPair_inv G)
   | TSplit a t' => fun G => interpret_split a (interpret_term2_dep rec (GTSplit_inv G))
-  | TInl a => fun G => interpret_inl a >>= interpret_kont1_dep rec (GTInl_inv G)
-  | TInr a => fun G => interpret_inr a >>= interpret_kont1_dep rec (GTInr_inv G)
+  | TInl a => fun G => interpret_inl a >>= interpret_kont_dep rec (GTInl_inv G)
+  | TInr a => fun G => interpret_inr a >>= interpret_kont_dep rec (GTInr_inv G)
   | TCase a t1 t2 => fun G => interpret_case a (interpret_term1_dep rec (GTCase_inv1 G)) (interpret_term1_dep rec (GTCase_inv2 G))
-  | TRef a => fun G => interpret_ref a >>= interpret_kont1_dep rec (GTRef_inv G)
-  | TGet a => fun G => interpret_get a >>= interpret_kont1_dep rec (GTGet_inv G)
-  | TSet a1 a2 => fun G => interpret_set a1 a2 >>= interpret_kont1_dep rec (GTSet_inv G)
-  | TFree a => fun G => interpret_free a >>= interpret_kont1_dep rec (GTFree_inv G)
+  | TRef a => fun G => interpret_ref a >>= interpret_kont_dep rec (GTRef_inv G)
+  | TGet a => fun G => interpret_get a >>= interpret_kont_dep rec (GTGet_inv G)
+  | TSet a1 a2 => fun G => interpret_set a1 a2 >>= interpret_kont_dep rec (GTSet_inv G)
+  | TFree a => fun G => interpret_free a >>= interpret_kont_dep rec (GTFree_inv G)
   | TShift t' => fun G => interpret_shift k (fun env => interpret_clo1_dep rec (GTShift_inv G env))
-  | TReset t' => fun G => interpret_reset k (interpret_term_dep rec (GTReset_inv1 G)) (interpret_kont1_dep rec (GTReset_inv2 G))
+  | TReset t' => fun G => interpret_reset k (interpret_term_dep rec (GTReset_inv1 G)) (interpret_kont_dep rec (GTReset_inv2 G))
   | TControl t' => fun G => interpret_control k (fun env => interpret_clo1_dep rec (GTControl_inv G env))
-  | TPrompt t' => fun G => interpret_prompt k (interpret_term_dep rec (GTPrompt_inv1 G)) (interpret_kont1_dep rec (GTPrompt_inv2 G))
-  | TExn tag a => fun G => interpret_exn tag a >>= interpret_kont1_dep rec (GTExn_inv G)
+  | TPrompt t' => fun G => interpret_prompt k (interpret_term_dep rec (GTPrompt_inv1 G)) (interpret_kont_dep rec (GTPrompt_inv2 G))
+  | TExn tag a => fun G => interpret_exn tag a >>= interpret_kont_dep rec (GTExn_inv G)
   | TRaise a => fun G => interpret_raise a
-  | TTry t1 t2 => fun G => interpret_try k (interpret_term_dep rec (GTTry_inv1 G)) (interpret_kont1_dep rec (GTTry_inv2 G)) t2 (interpret_exn_term_dep rec (GTTry_inv3 G))
+  | TTry t1 t2 => fun G => interpret_try k t2
+                             (interpret_term_dep rec (GTTry_inv1 G))
+                             (interpret_kont_dep rec (GTTry_inv2 G))
+                             (interpret_exn_term_dep rec (GTTry_inv3 G))
   end G
-with interpret_term1_dep (rec : interpreter) (k : kont1) (t : term1) (G : term1_graph k t) (v : val) : imonad iresult :=
+with interpret_term1_dep (rec : interpreter) (k : kont) (t : term1) (G : term1_graph k t) (v : val) : imonad iresult :=
   match t return term1_graph k t -> imonad iresult with
   | T1 b t' => fun G => with_binder b v (interpret_term_dep rec (GT1_inv G))
   end G
-with interpret_term2_dep (rec : interpreter) (k : kont1) (t : term2) (G : term2_graph k t) (v1 v2 : val) : imonad iresult :=
+with interpret_term2_dep (rec : interpreter) (k : kont) (t : term2) (G : term2_graph k t) (v1 v2 : val) : imonad iresult :=
   match t return term2_graph k t -> imonad iresult with
   | T2 b1 b2 t' => fun G => with_binder b1 v1 (with_binder b2 v2 (interpret_term_dep rec (GT2_inv G)))
   end G
-with interpret_exn_term_dep (rec : interpreter) (k : kont1) (t : exn_term) (G : exn_term_graph k t) (exn : exn) : imonad iresult :=
+with interpret_exn_term_dep (rec : interpreter) (k : kont) (t : exn_term) (G : exn_term_graph k t) (exn : exn) : imonad iresult :=
   match t return exn_term_graph k t -> imonad iresult with
-  | ExnT p t' => fun G => with_exn_pattern p exn (interpret_term_dep rec (GExnT_inv G))
+  | ExnTBase p t' => fun G => with_exn_pattern p exn (interpret_term_dep rec (GExnTBase_inv G)) (imonad_pure (RRaise exn))
+  | ExnTCons p t1 t2 => fun G => with_exn_pattern p exn (interpret_term_dep rec (GExnTCons_inv1 G)) (interpret_exn_term_dep rec (GExnTCons_inv2 G) exn)
   end G
-with interpret_clo1_dep (rec : interpreter) (k : kont1) (c : clo1) (G : clo1_graph k c) (v : val) : imonad iresult :=
+with interpret_clo1_dep (rec : interpreter) (k : kont) (c : clo1) (G : clo1_graph k c) (v : val) : imonad iresult :=
   match c return clo1_graph k c -> imonad iresult with
   | C1 env t => fun G => imonad_local_env (fun _ => env) (interpret_term1_dep rec (GC1_inv G) v)
   end G
-with interpret_kont1_dep (rec : interpreter) (k : kont1) (G : kont1_graph k) (v : val) : imonad iresult :=
-  match k return kont1_graph k -> imonad iresult with
-  | K1Nil => fun _ => imonad_pure (RReturn v)
-  | K1Cons c k' => fun G => interpret_clo1_dep rec (GK1Cons_inv G) v
+with interpret_kont_dep (rec : interpreter) (k : kont) (G : kont_graph k) (v : val) : imonad iresult :=
+  match k return kont_graph k -> imonad iresult with
+  | KNil => fun G => imonad_pure (RReturn v)
+  | KCons c k' => fun G => interpret_clo1_dep rec (GKCons_inv G) v
   end G.
 
 Unset Implicit Arguments.
 
-Fixpoint build_kont1_graph (k : kont1) : kont1_graph k :=
+Fixpoint build_kont_graph (k : kont) : kont_graph k :=
   match k with
-  | K1Nil => GK1Nil
-  | K1Cons c k' => GK1Cons (build_clo1_graph_dep (build_kont1_graph k') c)
+  | KNil => GKNil
+  | KCons c k' => GKCons (build_clo1_graph_dep (build_kont_graph k') c)
   end.
 
-Definition build_term_graph (k : kont1) (t : term) : term_graph k t :=
-  build_term_graph_dep (build_kont1_graph k) t.
+Definition build_term_graph (k : kont) (t : term) : term_graph k t :=
+  build_term_graph_dep (build_kont_graph k) t.
 
-Definition interpret_term_aux (rec : interpreter) (k : kont1) (t : term) : imonad iresult :=
+Definition interpret_term_aux (rec : interpreter) (k : kont) (t : term) : imonad iresult :=
   interpret_term_dep rec (build_term_graph k t).
 
-Fixpoint interpret_term (fuel : nat) (k : kont1) (t : term) : imonad iresult :=
+Fixpoint interpret_term (fuel : nat) (k : kont) (t : term) : imonad iresult :=
   match fuel with
   | O => imonad_throw OutOfFuel
   | S fuel' => interpret_term_aux (interpret_term fuel') k t
   end.
 
 Definition run_term (fuel : nat) (t : term) : (ierror + val) * iheap :=
-  imonad_run (interpret_term fuel K1Nil t >>= unwrap_RReturn) EnvNil iheap_empty.
+  imonad_run (interpret_term fuel KNil t >>= unwrap_RReturn) EnvNil iheap_empty.
 
 Definition eval_term (fuel : nat) (t : term) : ierror + val :=
   fst (run_term fuel t).
