shift-reset/core/syntax.v
@@ -31,10 +31,10 @@ Inductive binder : Type :=
 | BAny : binder
 | BVar : var -> binder.
 
-Inductive exn_pattern : Type :=
-| ExnPAny : exn_pattern
-| ExnPVar : var -> exn_pattern
-| ExnPTag : tag -> var -> exn_pattern.
+Inductive pattern : Type :=
+| PAny : pattern
+| PVar : var -> pattern
+| PTag : tag -> binder -> pattern.
 
 Inductive term : Type :=
 | TAtom : atom -> term
@@ -66,7 +66,8 @@ with term1 : Type :=
 with term2 : Type :=
 | T2 : binder -> binder -> term -> term2
 with exn_term : Type :=
-| ExnT : exn_pattern -> term -> exn_term.
+| ExnTBase : pattern -> term -> exn_term
+| ExnTCons : pattern -> term -> exn_term -> exn_term.
 
 Inductive val : Type :=
 | VUnit : val
@@ -78,8 +79,8 @@ Inductive val : Type :=
 | VInl : val -> val
 | VInr : val -> val
 | VLoc : loc -> val
-| VKontS : kont2S -> val
-| VKontC : kont2C -> val
+| VKontReset : metakont -> val
+| VKont : metakont -> val
 | VExn : exn -> val
 with clo1 : Type :=
 | C1 : env -> term1 -> clo1
@@ -87,17 +88,14 @@ with clo2 : Type :=
 | C2 : env -> term2 -> clo2
 with exn_clo : Type :=
 | ExnC : env -> exn_term -> exn_clo
-with kont1 : Type :=
-| K1Nil : kont1
-| K1Cons : clo1 -> kont1 -> kont1
-with kont2S : Type :=
-| K2SPure : kont1 -> kont2S
-| K2SPrompt : kont2S -> kont1 -> kont2S
-| K2STry : kont2S -> exn_clo -> kont1 -> kont2S
-with kont2C : Type :=
-| K2CPure : kont1 -> kont2C
-| K2CReset : kont2C -> kont1 -> kont2C
-| K2CTry : kont2C -> exn_clo -> kont1 -> kont2C
+with kont : Type :=
+| KNil : kont
+| KCons : clo1 -> kont -> kont
+with metakont : Type :=
+| MKPure : kont -> metakont
+| MKReset : metakont -> kont -> metakont
+| MKPrompt : metakont -> kont -> metakont
+| MKTry : metakont -> exn_clo -> kont -> metakont
 with env : Type :=
 | EnvNil : env
 | EnvCons : var -> val -> env -> env
@@ -124,14 +122,15 @@ Proof. decide equality; auto with eq_dec_db. Defined.
 Definition binder_eq_dec : forall (b1 b2 : binder), {b1 = b2} + {b1 <> b2}.
 Proof. decide equality; auto with eq_dec_db. Defined.
 
-Definition exn_pattern_eq_dec : forall (p1 p2 : exn_pattern), {p1 = p2} + {p1 <> p2}.
-Proof. decide equality; auto with eq_dec_db. Defined.
-
 Hint Resolve prim1_eq_dec : eq_dec_db.
 Hint Resolve prim2_eq_dec : eq_dec_db.
 Hint Resolve atom_eq_dec : eq_dec_db.
 Hint Resolve binder_eq_dec : eq_dec_db.
-Hint Resolve exn_pattern_eq_dec : eq_dec_db.
+
+Definition pattern_eq_dec : forall (p1 p2 : pattern), {p1 = p2} + {p1 <> p2}.
+Proof. decide equality; auto with eq_dec_db. Defined.
+
+Hint Resolve pattern_eq_dec : eq_dec_db.
 
 Fixpoint term_eq_dec : forall (t1 t2 : term), {t1 = t2} + {t1 <> t2}
 with term1_eq_dec : forall (t1 t2 : term1), {t1 = t2} + {t1 <> t2}
@@ -148,9 +147,8 @@ Fixpoint val_eq_dec : forall (v1 v2 : val), {v1 = v2} + {v1 <> v2}
 with clo1_eq_dec : forall (c1 c2 : clo1), {c1 = c2} + {c1 <> c2}
 with clo2_eq_dec : forall (c1 c2 : clo2), {c1 = c2} + {c1 <> c2}
 with exn_clo_eq_dec : forall (c1 c2 : exn_clo), {c1 = c2} + {c1 <> c2}
-with kont1_eq_dec : forall (k1 k2 : kont1), {k1 = k2} + {k1 <> k2}
-with kont2S_eq_dec : forall (ks1 ks2 : kont2S), {ks1 = ks2} + {ks1 <> ks2}
-with kont2C_eq_dec : forall (kc1 kc2 : kont2C), {kc1 = kc2} + {kc1 <> kc2}
+with kont_eq_dec : forall (k1 k2 : kont), {k1 = k2} + {k1 <> k2}
+with metakont_eq_dec : forall (mk1 mk2 : metakont), {mk1 = mk2} + {mk1 <> mk2}
 with env_eq_dec : forall (env1 env2 : env), {env1 = env2} + {env1 <> env2}
 with exn_eq_dec : forall (exn1 exn2 : exn), {exn1 = exn2} + {exn1 <> exn2}.
 Proof. all: decide equality; auto with eq_dec_db. Defined.
@@ -159,9 +157,8 @@ Hint Resolve val_eq_dec : eq_dec_db.
 Hint Resolve clo1_eq_dec : eq_dec_db.
 Hint Resolve clo2_eq_dec : eq_dec_db.
 Hint Resolve exn_clo_eq_dec : eq_dec_db.
-Hint Resolve kont1_eq_dec : eq_dec_db.
-Hint Resolve kont2S_eq_dec : eq_dec_db.
-Hint Resolve kont2C_eq_dec : eq_dec_db.
+Hint Resolve kont_eq_dec : eq_dec_db.
+Hint Resolve metakont_eq_dec : eq_dec_db.
 Hint Resolve env_eq_dec : eq_dec_db.
 Hint Resolve exn_eq_dec : eq_dec_db.
 
@@ -172,6 +169,7 @@ Module Coerce.
   Coercion Tag : string >-> tag.
   Coercion Var : string >-> var.
   Coercion BVar : var >-> binder.
+  Coercion PVar : var >-> pattern.
   Coercion AInt : Z >-> atom.
   Coercion ABool : bool >-> atom.
   Coercion AVar : var >-> atom.
